src/definitions/SharedLogic.v
@@ -7,10 +7,6 @@ Variant polarity : Type :=
 | Pos : polarity
 | Neg : polarity.
 
-Lemma polarity_eq_dec : forall p1 p2 : polarity, {p1 = p2} + {p1 <> p2}.
-Proof. decide equality. Defined
-.
-
 Inductive o : Type :=
 | Atom  : polarity -> nat -> o   
 | TT  : o
@@ -19,13 +15,6 @@ Inductive o : Type :=
 | AndN  : o -> o -> o
 | Or    : o -> o -> o
 | Imp  : o -> o -> o.
-
-Lemma o_eq_dec : forall A B : o, {A = B} + {A <> B}.
-Proof.
-  decide equality.
-  - apply Nat.eq_dec.
-  - apply polarity_eq_dec.
-Defined.
 
 Variant atomic : o -> Prop :=
   | Is_atom : forall p n, atomic (Atom p n)
@@ -58,3 +47,7 @@ Variant permeable : o -> Prop :=
 Notation sctx := (list o).
 Notation lctx := (list o).
 Notation octx := (list o).
+
+Definition permeable_ctx (C : sctx) : Prop := Forall permeable C.
+
+
