src/definitions/Decidability.v
@@ -1,0 +1,35 @@
+From Stdlib Require Import List PeanoNat.
+From LJF Require Import SharedLogic.
+
+Lemma polarity_eq_dec : forall p1 p2 : polarity, {p1 = p2} + {p1 <> p2}.
+Proof. decide equality. Defined
+.
+
+Lemma o_eq_dec : forall A B : o, {A = B} + {A <> B}.
+Proof.
+  decide equality.
+  - apply Nat.eq_dec.
+  - apply polarity_eq_dec.
+Defined.
+
+Lemma permeable_dec : forall A : o, {permeable A} + {~ permeable A}.
+Proof.
+    intros. destruct A.
+    - destruct p.
+        + left. apply Permeable_pos_atom. apply Is_atom. apply Pos_atom.
+        + left. apply Permeable_neg. apply Neg_atom.
+    - right. intro. inversion H. inversion H0. inversion H0.
+    - right. intro. inversion H. inversion H0. inversion H0.
+    - right. intro. inversion H. inversion H0. inversion H0.
+    - left. apply Permeable_neg. apply Neg_and.
+    - right. intro. inversion H. inversion H0. inversion H0.
+    - left. apply Permeable_neg. apply Neg_imp.
+Defined.
+
+Lemma permeable_ctx_dec : forall (C: sctx), {permeable_ctx C} + {~ permeable_ctx C}.
+Proof.
+    intros.
+    apply Forall_dec.
+    apply permeable_dec.
+Defined.
+    
