src/metatheory/LJFPS/LJFPS_Completeness.v
@@ -1,0 +1,34 @@
+From Stdlib Require Import List Permutation.
+
+From LJF Require Import SharedLogic LJFPS_Rules LJFC_Rules Schemes.
+
+Theorem LJFC_completeness :
+    (forall {C: sctx} {L: octx} {K: o}, bctO C L K -> bct (mk_ndctx C) L K) /\
+    (forall {C: sctx} {L: octx} {K: o}, eptO C L K -> ept (mk_ndctx C) L K) /\
+    (forall {C: sctx} {N K: o}, lfcO C N K -> lfc (mk_ndctx C) N K) /\
+    (forall {C: sctx} {K: o}, rfcO C K -> rfc (mk_ndctx C) K).
+Proof.
+    apply LJFPS_mutind_all ; intros.
+    - apply bct_boxR. apply b. apply H.
+    - apply bct_AndNR. apply H. apply H0.
+    - apply bct_ImpR. apply H.
+    - eapply ept_Lf. apply nodup_In. apply i. apply b. apply n. apply H.
+    - apply ept_Rf. apply p. apply H.
+    - apply ept_boxL. apply b. apply p.
+        rewrite ndctx_insert_mk_ndctx_eq. apply H.
+    - apply ept_AndPL. apply b. apply H.
+    - apply ept_OrL. apply b. apply H. apply H0.
+    - apply ept_TrueL. apply b. apply H.
+    - apply ept_FalseL. apply b.
+    - apply lfc_Rl. apply b. apply p. apply H.
+    - apply lfc_Il. apply n. apply a.
+    - apply lfc_AndNL_1. apply b. apply H.
+    - apply lfc_AndNL_2. apply b. apply H.
+    - apply lfc_ImpL. apply b. apply H. apply H0.
+    - apply rfc_Rr. apply n. apply H.
+    - apply rfc_Ir. apply nodup_In. apply i. apply p. apply a.
+    - apply rfc_AndPR. apply H. apply H0.
+    - apply rfc_OrR_1. apply H.
+    - apply rfc_OrR_2. apply H.
+    - apply rfc_TrueR.
+Qed.
