src/metatheory/LJFPS/LJFPS_Exchange.v
@@ -4,56 +4,56 @@ From Stdlib Require Import Wellfounded Nat Arith Lia.
 From LJF Require Import SharedLogic Measures LJFC_Rules Schemes.
 
 Theorem LJFC_exchange_structural :
-  (forall {C: ndctx} {L: octx} {K: o}, bctC C L K -> forall {C': ndctx}, Permutation C C' -> bctC C' L K) /\
-  (forall {C: ndctx} {L: octx} {K: o}, eptC C L K -> forall {C': ndctx}, Permutation C C' -> eptC C' L K) /\
-  (forall {C: ndctx} {N K: o}, lfcC C N K -> forall {C': ndctx}, Permutation C C' -> lfcC C' N K) /\
-  (forall {C: ndctx} {P: o}, rfcC C P -> forall {C': ndctx}, Permutation C C' -> rfcC C' P). 
+  (forall {C: ndctx} {L: octx} {K: o}, bct C L K -> forall {C': ndctx}, Permutation C C' -> bct C' L K) /\
+  (forall {C: ndctx} {L: octx} {K: o}, ept C L K -> forall {C': ndctx}, Permutation C C' -> ept C' L K) /\
+  (forall {C: ndctx} {N K: o}, lfc C N K -> forall {C': ndctx}, Permutation C C' -> lfc C' N K) /\
+  (forall {C: ndctx} {P: o}, rfc C P -> forall {C': ndctx}, Permutation C C' -> rfc C' P). 
 Proof.
     apply LJFC_mutind_all ; intros.
-        - apply bctC_boxR. apply b. apply H. apply H0.
-        - apply bctC_AndNR. apply H. apply H1. apply H0. apply H1.
-        - apply bctC_ImpR. apply H. apply H0.
-        - eapply eptC_Lf. eapply Permutation_in. apply H0. apply i. apply b. apply n. apply H. apply H0.
-        - apply eptC_Rf. apply p. apply H. apply H0.
-        - apply eptC_boxL. apply b. apply p. apply H.
+        - apply bct_boxR. apply b. apply H. apply H0.
+        - apply bct_AndNR. apply H. apply H1. apply H0. apply H1.
+        - apply bct_ImpR. apply H. apply H0.
+        - eapply ept_Lf. eapply Permutation_in. apply H0. apply i. apply b. apply n. apply H. apply H0.
+        - apply ept_Rf. apply p. apply H. apply H0.
+        - apply ept_boxL. apply b. apply p. apply H.
           apply ndctx_insert_perm_cons. apply H0.
-        - apply eptC_AndPL. apply b. apply H. apply H0.
-        - apply eptC_OrL. apply b. apply H. apply H1. apply H0. apply H1.
-        - apply eptC_TrueL. apply b. apply H. apply H0.
-        - apply eptC_FalseL. apply b.
-        - apply lfcC_Rl. apply b. apply p. apply H. apply H0.
-        - apply lfcC_Il. apply n. apply a.
-        - apply lfcC_AndNL_1. apply b. apply H. apply H0.
-        - apply lfcC_AndNL_2. apply b. apply H. apply H0.
-        - apply lfcC_ImpL. apply b. apply H. apply H1. apply H0. apply H1.
-        - apply rfcC_Rr. apply n. apply H. apply H0.
-        - apply rfcC_Ir. eapply Permutation_in. apply H. apply i. apply p. apply a.
-        - apply rfcC_AndPR. apply H. apply H1. apply H0. apply H1.
-        - apply rfcC_OrR_1. apply H. apply H0.
-        - apply rfcC_OrR_2. apply H. apply H0.
-        - apply rfcC_TrueR.
+        - apply ept_AndPL. apply b. apply H. apply H0.
+        - apply ept_OrL. apply b. apply H. apply H1. apply H0. apply H1.
+        - apply ept_TrueL. apply b. apply H. apply H0.
+        - apply ept_FalseL. apply b.
+        - apply lfc_Rl. apply b. apply p. apply H. apply H0.
+        - apply lfc_Il. apply n. apply a.
+        - apply lfc_AndNL_1. apply b. apply H. apply H0.
+        - apply lfc_AndNL_2. apply b. apply H. apply H0.
+        - apply lfc_ImpL. apply b. apply H. apply H1. apply H0. apply H1.
+        - apply rfc_Rr. apply n. apply H. apply H0.
+        - apply rfc_Ir. eapply Permutation_in. apply H. apply i. apply p. apply a.
+        - apply rfc_AndPR. apply H. apply H1. apply H0. apply H1.
+        - apply rfc_OrR_1. apply H. apply H0.
+        - apply rfc_OrR_2. apply H. apply H0.
+        - apply rfc_TrueR.
 Qed.
 
-Lemma LJFC_exchange_structural_bctC :
-    forall {C: ndctx} {L: octx} {K: o}, bctC C L K -> forall {C': ndctx}, Permutation C C' -> bctC C' L K.
+Lemma LJFC_exchange_structural_bct :
+    forall {C: ndctx} {L: octx} {K: o}, bct C L K -> forall {C': ndctx}, Permutation C C' -> bct C' L K.
 Proof.
   destruct LJFC_exchange_structural. apply H.
 Qed.
 
-Lemma LJFC_exchange_structural_eptC :
-    forall {C: ndctx} {L: octx} {K: o}, eptC C L K -> forall {C': ndctx}, Permutation C C' -> eptC C' L K.
+Lemma LJFC_exchange_structural_ept :
+    forall {C: ndctx} {L: octx} {K: o}, ept C L K -> forall {C': ndctx}, Permutation C C' -> ept C' L K.
 Proof.
   destruct LJFC_exchange_structural. destruct H0. apply H0.
 Qed.
 
-Lemma LJFC_exchange_structural_lfcC :
-  forall {C: ndctx} {N K: o}, lfcC C N K -> forall {C': ndctx}, Permutation C C' -> lfcC C' N K.
+Lemma LJFC_exchange_structural_lfc :
+  forall {C: ndctx} {N K: o}, lfc C N K -> forall {C': ndctx}, Permutation C C' -> lfc C' N K.
 Proof.
   destruct LJFC_exchange_structural. destruct H0. destruct H1. apply H1.
 Qed.
 
-Lemma LJFC_exchange_structural_rfcC :
-  forall {C: ndctx} {K: o}, rfcC C K -> forall {C': ndctx}, Permutation C C' -> rfcC C' K.
+Lemma LJFC_exchange_structural_rfc :
+  forall {C: ndctx} {K: o}, rfc C K -> forall {C': ndctx}, Permutation C C' -> rfc C' K.
 Proof.
   destruct LJFC_exchange_structural. destruct H0. destruct H1. apply H2.
 Qed.
@@ -62,31 +62,31 @@ Lemma eager_boxL :
   forall {C0: ndctx} {L: octx} {B: o} {K: o},
     bracketable K ->
     permeable B ->
-    eptC C0 L K ->
+    ept C0 L K ->
     forall {C: ndctx} {L1 L2: octx},
       Permutation C0 (ndctx_insert B C) ->
       L = L1 ++ L2 ->
-      eptC C (L1 ++ B :: L2) K.
+      ept C (L1 ++ B :: L2) K.
 Proof.
   intros C0 L B K b p H ; induction H ; intros.
     - symmetry in H4. apply app_eq_nil in H4. destruct H4. subst. simpl.
-      apply eptC_boxL. apply b. apply p.
-      eapply eptC_Lf. eapply Permutation_in.
+      apply ept_boxL. apply b. apply p.
+      eapply ept_Lf. eapply Permutation_in.
         unfold ndctx_list in *.
         apply H3. apply H. apply b. apply H1.
-      eapply LJFC_exchange_structural_lfcC. apply H2. apply H3.
+      eapply LJFC_exchange_structural_lfc. apply H2. apply H3.
     - symmetry in H2. apply app_eq_nil in H2. destruct H2. subst. simpl.
-      apply eptC_boxL. apply b. apply p.
-      apply eptC_Rf. apply H. 
-      eapply LJFC_exchange_structural_rfcC. apply H0. apply H1.
+      apply ept_boxL. apply b. apply p.
+      apply ept_Rf. apply H. 
+      eapply LJFC_exchange_structural_rfc. apply H0. apply H1.
     - symmetry in H3. apply app_eq_cons in H3. destruct H3. 
       + destruct H3. subst. simpl.
-        apply eptC_boxL. apply b. apply p. 
-        eapply LJFC_exchange_structural_eptC. 2: apply H2.
-        apply eptC_boxL. apply H. apply H0. apply H1.
+        apply ept_boxL. apply b. apply p. 
+        eapply LJFC_exchange_structural_ept. 2: apply H2.
+        apply ept_boxL. apply H. apply H0. apply H1.
       + destruct H3. destruct H3. subst. simpl. 
-        apply eptC_boxL. apply H. apply H0.
-        apply IHeptC. apply H.
+        apply ept_boxL. apply H. apply H0.
+        apply IHept. apply H.
         apply Permutation_sym.
         apply ndctx_insert_perm_swap.
         apply ndctx_insert_perm_cons.
@@ -94,92 +94,92 @@ Proof.
         apply H2.
         reflexivity.
     - symmetry in H2. apply app_eq_cons in H2. destruct H2 ; destruct H2.
-      + subst. simpl. apply eptC_boxL. apply b. apply p.
-        apply eptC_AndPL. apply b.
-        eapply LJFC_exchange_structural_eptC. apply H0. apply H1.
+      + subst. simpl. apply ept_boxL. apply b. apply p.
+        apply ept_AndPL. apply b.
+        eapply LJFC_exchange_structural_ept. apply H0. apply H1.
       + destruct H2. subst. simpl.
-        apply eptC_AndPL. apply H.
-        eapply IHeptC with (L1 := B2 :: B1 :: x). apply b. apply H1. reflexivity.
+        apply ept_AndPL. apply H.
+        eapply IHept with (L1 := B2 :: B1 :: x). apply b. apply H1. reflexivity.
     - symmetry in H3. apply app_eq_cons in H3. destruct H3 ; destruct H3.
       + subst. simpl.
-        apply eptC_boxL. apply b. apply p.
-        apply eptC_OrL. apply b.
-          -- eapply LJFC_exchange_structural_eptC. apply H0. apply H2.
-          -- eapply LJFC_exchange_structural_eptC. apply H1. apply H2.
+        apply ept_boxL. apply b. apply p.
+        apply ept_OrL. apply b.
+          -- eapply LJFC_exchange_structural_ept. apply H0. apply H2.
+          -- eapply LJFC_exchange_structural_ept. apply H1. apply H2.
       + destruct H3. subst. simpl. 
-        apply eptC_OrL. apply b.
-          -- eapply IHeptC1 with (L1 := B1 :: x). apply b. apply H2. reflexivity.
-          -- eapply IHeptC2 with (L1 := B2 :: x). apply b. apply H2. reflexivity.
+        apply ept_OrL. apply b.
+          -- eapply IHept1 with (L1 := B1 :: x). apply b. apply H2. reflexivity.
+          -- eapply IHept2 with (L1 := B2 :: x). apply b. apply H2. reflexivity.
     - symmetry in H2. apply app_eq_cons in H2. destruct H2 ; destruct H2.
-      + subst. simpl. apply eptC_boxL. apply b. apply p.
-        apply eptC_TrueL. apply b.
-        eapply LJFC_exchange_structural_eptC. apply H0. apply H1.
+      + subst. simpl. apply ept_boxL. apply b. apply p.
+        apply ept_TrueL. apply b.
+        eapply LJFC_exchange_structural_ept. apply H0. apply H1.
       + destruct H2. subst. simpl.
-        apply eptC_TrueL. apply H.
-        eapply IHeptC with (L1 := x). apply b. apply H1. reflexivity.
+        apply ept_TrueL. apply H.
+        eapply IHept with (L1 := x). apply b. apply H1. reflexivity.
     - symmetry in H1. apply app_eq_cons in H1. destruct H1 ; destruct H1.
-      + subst. simpl. apply eptC_boxL. apply b. apply p.
-        apply eptC_FalseL. apply b.
+      + subst. simpl. apply ept_boxL. apply b. apply p.
+        apply ept_FalseL. apply b.
       + destruct H1. subst. simpl.
-        apply eptC_FalseL. apply H.
+        apply ept_FalseL. apply H.
 Qed.        
         
 Lemma eager_AndPL :
   forall {C: ndctx} {L: octx} {B1 B2 K: o},
     bracketable K ->
-    eptC C L K ->
+    ept C L K ->
       forall {L1 L2: octx},
       L = L1 ++ B2 :: B1 :: L2 ->
-      eptC C (L1 ++ (AndP B1 B2) :: L2) K.
+      ept C (L1 ++ (AndP B1 B2) :: L2) K.
 Proof.
   intros C L B1 B2 K b H. induction H ; intros L1 L2 Ho.
     - symmetry in Ho. apply app_eq_nil in Ho. destruct Ho. discriminate H4.
     - symmetry in Ho. apply app_eq_nil in Ho. destruct Ho. discriminate H2.
     - symmetry in Ho. apply app_eq_cons in Ho. destruct Ho.
       + destruct H2. inversion H3. subst. clear H3. simpl.
-        apply eptC_AndPL. apply H.
-        apply eptC_boxL. apply H. apply H0. apply H1. 
+        apply ept_AndPL. apply H.
+        apply ept_boxL. apply H. apply H0. apply H1. 
       + destruct H2. destruct H2. subst. simpl.
-        apply eptC_boxL. apply H. apply H0. 
-        apply IHeptC. apply H. reflexivity.
+        apply ept_boxL. apply H. apply H0. 
+        apply IHept. apply H. reflexivity.
     - symmetry in Ho. apply app_eq_cons in Ho. destruct Ho.
       + destruct H1. inversion H2. subst. simpl.
-        apply eptC_AndPL. apply H. 
-        apply eptC_AndPL. apply H. apply H0. 
+        apply ept_AndPL. apply H. 
+        apply ept_AndPL. apply H. apply H0. 
       + destruct H1. destruct H1. subst. simpl.
-        apply eptC_AndPL. apply H.
-        apply IHeptC with (L1 := B3 :: B0 :: x). apply b. reflexivity.
+        apply ept_AndPL. apply H.
+        apply IHept with (L1 := B3 :: B0 :: x). apply b. reflexivity.
     - symmetry in Ho. apply app_eq_cons in Ho. destruct Ho.
       + destruct H2. inversion H3. subst. simpl. clear H3.
-        apply eptC_AndPL. apply H. 
-        apply eptC_OrL. apply H. apply H0. apply H1.
+        apply ept_AndPL. apply H. 
+        apply ept_OrL. apply H. apply H0. apply H1.
       + destruct H2. destruct H2. subst. simpl.
-        apply eptC_OrL. apply H.
-        -- apply IHeptC1 with (L1 := (B0 :: x)). apply H. reflexivity.
-        -- apply IHeptC2 with (L1 := (B3 :: x)). apply H. reflexivity.
+        apply ept_OrL. apply H.
+        -- apply IHept1 with (L1 := (B0 :: x)). apply H. reflexivity.
+        -- apply IHept2 with (L1 := (B3 :: x)). apply H. reflexivity.
     - symmetry in Ho. apply app_eq_cons in Ho. destruct Ho.
       + destruct H1. inversion H2. subst. simpl.
-        apply eptC_AndPL. apply H.
-        apply eptC_TrueL. apply H.
+        apply ept_AndPL. apply H.
+        apply ept_TrueL. apply H.
         apply H0.
       + destruct H1. destruct H1. subst. simpl.
-        apply eptC_TrueL. apply H. 
-        apply IHeptC. apply H. reflexivity.
+        apply ept_TrueL. apply H. 
+        apply IHept. apply H. reflexivity.
     - symmetry in Ho. apply app_eq_cons in Ho. destruct Ho.
       + destruct H0. inversion H1. subst. simpl. 
-        apply eptC_AndPL. apply H. apply eptC_FalseL. apply H.
+        apply ept_AndPL. apply H. apply ept_FalseL. apply H.
       + destruct H0. destruct H0. subst. simpl.
-        apply eptC_FalseL. apply H.
+        apply ept_FalseL. apply H.
 Qed.
 
 Lemma LJFC_inversion_boxL :
   forall {C: ndctx} {L: octx} {B K: o},
     bracketable K ->
     permeable B ->
-    eptC C L K ->
+    ept C L K ->
     forall {L1: octx},
       L = B :: L1 ->  
-      eptC (ndctx_insert B C) L1 K.
+      ept (ndctx_insert B C) L1 K.
 Proof.
   intros C L B K b p H. induction H ; intros L1 Ho.
     - discriminate Ho.
@@ -194,13 +194,13 @@ Qed.
 Lemma eager_OrL :
   forall {C: ndctx} {L: octx} {B1 B2 K: o},
     bracketable K ->
-    eptC C L K ->
+    ept C L K ->
     forall {L' : octx},
-      eptC C L' K ->
+      ept C L' K ->
       forall {L1 L2: octx},
         L = L1 ++ B1 :: L2 ->
         L' = L1 ++ B2 :: L2 ->
-        eptC C (L1 ++ (Or B1 B2) :: L2) K.
+        ept C (L1 ++ (Or B1 B2) :: L2) K.
 Proof.
   intros C L B1 B2 K b H. induction H ; intros L' H' L1 L2 Ho Ho'.
     - subst. symmetry in Ho. apply app_eq_nil in Ho. destruct Ho.
@@ -209,123 +209,123 @@ Proof.
       inversion H2.
     - subst. symmetry in Ho. apply app_eq_cons in Ho. destruct Ho.
       + destruct H2. inversion H3. subst. simpl. 
-        apply eptC_OrL. apply H.
-          -- apply eptC_boxL. apply H. apply H0. apply H1.
+        apply ept_OrL. apply H.
+          -- apply ept_boxL. apply H. apply H0. apply H1.
           -- apply H'.
       + destruct H2. destruct H2. subst. simpl.
-        apply eptC_boxL. apply H. apply H0.
+        apply ept_boxL. apply H. apply H0.
         simpl in H'.
-        eapply IHeptC with (L' := x ++ B2 :: L2). apply H.
+        eapply IHept with (L' := x ++ B2 :: L2). apply H.
         eapply LJFC_inversion_boxL. apply H. apply H0.
         apply H'. reflexivity. reflexivity. reflexivity.
     - symmetry in Ho. apply app_eq_cons in Ho. destruct Ho.
       + destruct H1. inversion H2. subst. simpl. 
-        apply eptC_OrL. apply H. apply eptC_AndPL. apply H. apply H0. apply H'.
+        apply ept_OrL. apply H. apply ept_AndPL. apply H. apply H0. apply H'.
       + destruct H1. destruct H1. subst.
-        simpl. apply eptC_AndPL. apply H.
-        eapply IHeptC with (L1 := B3 :: B0 :: x). apply H.
+        simpl. apply ept_AndPL. apply H.
+        eapply IHept with (L1 := B3 :: B0 :: x). apply H.
         inversion H'. subst. inversion H5. inversion H1. inversion H1. subst.
         apply H7. reflexivity. reflexivity.
     - subst. symmetry in Ho. apply app_eq_cons in Ho. destruct Ho.
       + destruct H2. inversion H3. subst. simpl.
-        apply eptC_OrL. apply H. apply eptC_OrL. apply H.
+        apply ept_OrL. apply H. apply ept_OrL. apply H.
         apply H0. apply H1. apply H'.
       + destruct H2. destruct H2. subst. simpl.
-        apply eptC_OrL. apply H. 
+        apply ept_OrL. apply H. 
         inversion H'. subst. inversion H6. inversion H2. inversion H2. subst.
-        eapply IHeptC1 with (L1 := B0 :: x). apply H. apply H8. reflexivity. reflexivity.
+        eapply IHept1 with (L1 := B0 :: x). apply H. apply H8. reflexivity. reflexivity.
         inversion H'. subst. inversion H6. inversion H2. inversion H2. subst.
-        eapply IHeptC2 with (L1 := B3 :: x). apply H. apply H9. reflexivity. reflexivity.
+        eapply IHept2 with (L1 := B3 :: x). apply H. apply H9. reflexivity. reflexivity.
     - symmetry in Ho. apply app_eq_cons in Ho. destruct Ho.
       + destruct H1. inversion H2. subst. simpl.
-        apply eptC_OrL. apply H.
-        apply eptC_TrueL. apply H. apply H0.
+        apply ept_OrL. apply H.
+        apply ept_TrueL. apply H. apply H0.
         apply H'.
       + destruct H1. destruct H1. subst. simpl.
-        apply eptC_TrueL. apply H.
-        eapply IHeptC. apply H.
+        apply ept_TrueL. apply H.
+        eapply IHept. apply H.
         inversion H'. subst. inversion H5. inversion H1. inversion H1.
         subst. apply H4. reflexivity. reflexivity.
     - symmetry in Ho. apply app_eq_cons in Ho. destruct Ho.
       + destruct H0. inversion H1. subst. simpl.
-        apply eptC_OrL. apply H. apply eptC_FalseL. apply H. apply H'.
-      + destruct H0. destruct H0. subst. simpl. apply eptC_FalseL. apply H.
+        apply ept_OrL. apply H. apply ept_FalseL. apply H. apply H'.
+      + destruct H0. destruct H0. subst. simpl. apply ept_FalseL. apply H.
 Qed. 
 
 Lemma eager_TrueL :
   forall {C: ndctx} {L: octx} {K: o},
     bracketable K ->
-    eptC C L K ->
+    ept C L K ->
     forall {L1 L2: octx},
       L = L1 ++ L2 ->
-      eptC C (L1 ++ TT :: L2) K.
+      ept C (L1 ++ TT :: L2) K.
 Proof.
   intros C L K b H. induction H ; intros L1 L2 Ho.
     - symmetry in Ho. apply app_eq_nil in Ho. destruct Ho. subst. simpl.
-      apply eptC_TrueL. apply b. eapply eptC_Lf. apply H. apply H0.
+      apply ept_TrueL. apply b. eapply ept_Lf. apply H. apply H0.
       apply H1. apply H2.
     - symmetry in Ho. apply app_eq_nil in Ho. destruct Ho. subst. simpl.
-      apply eptC_TrueL. apply b. apply eptC_Rf. apply H. apply H0.
+      apply ept_TrueL. apply b. apply ept_Rf. apply H. apply H0.
     - destruct L1.
-      + simpl in Ho. subst. simpl. apply eptC_TrueL. apply H.
-        apply eptC_boxL. apply H. apply H0. apply H1.
+      + simpl in Ho. subst. simpl. apply ept_TrueL. apply H.
+        apply ept_boxL. apply H. apply H0. apply H1.
       + simpl in Ho. inversion Ho. subst. simpl.
-        apply eptC_boxL. apply H. apply H0.
-        apply IHeptC. apply H. reflexivity.
+        apply ept_boxL. apply H. apply H0.
+        apply IHept. apply H. reflexivity.
     - destruct L1.
-      + simpl in Ho. subst. simpl. apply eptC_TrueL. apply H.
-        apply eptC_AndPL. apply H. apply H0.
+      + simpl in Ho. subst. simpl. apply ept_TrueL. apply H.
+        apply ept_AndPL. apply H. apply H0.
       + simpl in Ho. inversion Ho. subst. simpl.
-        apply eptC_AndPL. apply H.
-        eapply IHeptC with (L1 := B2 :: B1 :: L1) (L2 := L2). apply H. reflexivity.
+        apply ept_AndPL. apply H.
+        eapply IHept with (L1 := B2 :: B1 :: L1) (L2 := L2). apply H. reflexivity.
     - destruct L1.
-      + simpl in Ho. subst. simpl. apply eptC_TrueL. apply H.
-        apply eptC_OrL. apply H. apply H0. apply H1.
+      + simpl in Ho. subst. simpl. apply ept_TrueL. apply H.
+        apply ept_OrL. apply H. apply H0. apply H1.
       + simpl in Ho. inversion Ho. subst. simpl.
-        apply eptC_OrL. apply H.
-        -- eapply IHeptC1 with (L1 := B1 :: L1). apply H. reflexivity.
-        -- eapply IHeptC2 with (L1 := B2 :: L1). apply H. reflexivity.
+        apply ept_OrL. apply H.
+        -- eapply IHept1 with (L1 := B1 :: L1). apply H. reflexivity.
+        -- eapply IHept2 with (L1 := B2 :: L1). apply H. reflexivity.
     - destruct L1.
-      + simpl in Ho. subst. simpl. apply eptC_TrueL. apply H.
-        apply eptC_TrueL. apply H. apply H0.
+      + simpl in Ho. subst. simpl. apply ept_TrueL. apply H.
+        apply ept_TrueL. apply H. apply H0.
       + simpl in Ho. inversion Ho. subst. simpl.
-        apply eptC_TrueL. apply H. apply IHeptC. apply H. reflexivity.
+        apply ept_TrueL. apply H. apply IHept. apply H. reflexivity.
     - destruct L1.
-      + simpl in Ho. subst. simpl. apply eptC_TrueL. apply H.
-        apply eptC_FalseL. apply H.
+      + simpl in Ho. subst. simpl. apply ept_TrueL. apply H.
+        apply ept_FalseL. apply H.
       + simpl in Ho. inversion Ho. subst. simpl.
-        apply eptC_FalseL. apply H.
+        apply ept_FalseL. apply H.
 Qed.
 
 Lemma eager_FalseL : 
   forall {C: ndctx} {L: octx} {K: o},
     bracketable K ->
     In FF L ->
-    eptC C L K.
+    ept C L K.
 Proof.
   intros C L K b. revert C.
   induction L using (well_founded_ind (wf_inverse_image octx nat lt octx_size PeanoNat.Nat.lt_wf_0)).
   destruct L ; intros C I. inversion I. destruct o.
-    + apply eptC_boxL. apply b. destruct p. 
+    + apply ept_boxL. apply b. destruct p. 
       apply Permeable_pos_atom. apply Is_atom. apply Pos_atom.
       apply Permeable_neg. apply Neg_atom. apply H.
       cbn [octx_size]. inversion I. discriminate H0.
       apply Nat.lt_add_pos_l. cbn [osize]. apply Nat.lt_0_1.
       inversion I. discriminate H0. apply H0.
-    + apply eptC_TrueL. apply b. apply H.
+    + apply ept_TrueL. apply b. apply H.
       cbn [octx_size]. inversion I. discriminate H0. 
       apply Nat.lt_add_pos_l. cbn [osize]. apply Nat.lt_0_1.
       inversion I. discriminate H0. apply H0.
-    + apply eptC_FalseL. apply b.
-    + apply eptC_AndPL. apply b. apply H.
+    + apply ept_FalseL. apply b.
+    + apply ept_AndPL. apply b. apply H.
       cbn [octx_size]. cbn [osize].
       simpl. rewrite Nat.add_shuffle3. rewrite Nat.add_assoc. apply Nat.lt_succ_diag_r.
       inversion I. discriminate H0. apply in_cons. apply in_cons. apply H0.
-    + apply eptC_boxL. apply b. apply Permeable_neg. apply Neg_and.
+    + apply ept_boxL. apply b. apply Permeable_neg. apply Neg_and.
       apply H. cbn [octx_size]. apply Nat.lt_add_pos_l. 
       cbn [osize]. apply Nat.lt_lt_add_r. apply Nat.lt_lt_add_r. apply Nat.lt_0_1.
       inversion I. discriminate H0. apply H0.
-    + apply eptC_OrL. apply b.
+    + apply ept_OrL. apply b.
       -- apply H. cbn [octx_size]. cbn [osize]. simpl.
         apply Nat.lt_succ_r.
         apply add_le_mono_r_proj_l2r. apply Nat.le_add_r.
@@ -334,7 +334,7 @@ Proof.
         apply Nat.lt_succ_r.
         apply add_le_mono_r_proj_l2r. apply Nat.le_add_l.
         inversion I. discriminate H0. apply in_cons. apply H0.
-    + apply eptC_boxL. apply b. apply Permeable_neg. apply Neg_imp.
+    + apply ept_boxL. apply b. apply Permeable_neg. apply Neg_imp.
       apply H. cbn [octx_size]. apply Nat.lt_add_pos_l. 
       cbn [osize]. apply Nat.lt_lt_add_r. apply Nat.lt_lt_add_r. apply Nat.lt_0_1.
       inversion I. discriminate H0. apply H0.
@@ -342,15 +342,15 @@ Qed.
 
 
 Theorem LJFC_exchange_ordered :
-  (forall {C: ndctx} {L: octx} {K: o}, bctC C L K -> forall {L': octx}, Permutation L L' -> bctC C L' K) /\
-  (forall {C: ndctx} {L: octx} {K: o}, eptC C L K -> forall {L': octx}, Permutation L L' -> eptC C L' K).
+  (forall {C: ndctx} {L: octx} {K: o}, bct C L K -> forall {L': octx}, Permutation L L' -> bct C L' K) /\
+  (forall {C: ndctx} {L: octx} {K: o}, ept C L K -> forall {L': octx}, Permutation L L' -> ept C L' K).
 Proof.
     apply LJFC_mutind_async ; intros.
-      - apply bctC_boxR. apply b. apply H. apply H0.
-      - apply bctC_AndNR. apply H. apply H1. apply H0. apply H1.
-      - apply bctC_ImpR. apply H. apply Permutation_cons. reflexivity. apply H0.
-      - apply Permutation_nil in H. subst. eapply eptC_Lf. apply i. apply b. apply n. apply l.
-      - apply Permutation_nil in H. subst. apply eptC_Rf. apply p. apply r.
+      - apply bct_boxR. apply b. apply H. apply H0.
+      - apply bct_AndNR. apply H. apply H1. apply H0. apply H1.
+      - apply bct_ImpR. apply H. apply Permutation_cons. reflexivity. apply H0.
+      - apply Permutation_nil in H. subst. eapply ept_Lf. apply i. apply b. apply n. apply l.
+      - apply Permutation_nil in H. subst. apply ept_Rf. apply p. apply r.
       - pose proof H0.
         symmetry in H1. apply Permutation_vs_cons_inv in H1. destruct H1. destruct H1. subst.
         eapply eager_boxL. apply b. apply p. 3: reflexivity. 2: apply Permutation_refl.
@@ -372,14 +372,14 @@ Proof.
         apply H. apply in_eq.
 Qed.
 
-Lemma LJFC_exchange_ordered_bctC :
-  forall {C: ndctx} {L: octx} {K: o}, bctC C L K -> forall {L': octx}, Permutation L L' -> bctC C L' K.
+Lemma LJFC_exchange_ordered_bct :
+  forall {C: ndctx} {L: octx} {K: o}, bct C L K -> forall {L': octx}, Permutation L L' -> bct C L' K.
 Proof.
   destruct LJFC_exchange_ordered. apply H.
 Qed.
 
-Lemma LJFC_exchange_ordered_eptC :
-  forall {C: ndctx} {L: octx} {K: o}, eptC C L K -> forall {L': octx}, Permutation L L' -> eptC C L' K.
+Lemma LJFC_exchange_ordered_ept :
+  forall {C: ndctx} {L: octx} {K: o}, ept C L K -> forall {L': octx}, Permutation L L' -> ept C L' K.
 Proof.
   destruct LJFC_exchange_ordered. apply H0.
 Qed.
