src/rules/LJFPS_Rules.v
@@ -1,0 +1,114 @@
+From Stdlib Require Import List Permutation ProofIrrelevance.
+From LJF Require Import SharedLogic.
+
+Inductive bct : ndctx -> octx -> o -> Prop :=
+| bct_boxR :
+  forall {C: ndctx} {L: octx} {D: o},
+    bracketable D ->
+    ept C L D ->
+    bct C L D
+| bct_AndNR :
+  forall {C: ndctx} {L: octx} {B1 B2: o},
+    bct C L B1 ->
+    bct C L B2 ->
+    bct C L (AndN B1 B2)
+| bct_ImpR :
+  forall {C: ndctx} {L: octx} {B1 B2: o},
+    bct C (B1 :: L) B2 ->
+    bct C L (Imp B1 B2)
+with ept : ndctx -> octx -> o -> Prop :=
+| ept_Lf :
+  forall {C: ndctx} (N : o) {K : o},
+    In N (ndctx_list C) ->
+    bracketable K ->
+    negative N ->
+    lfc C N K ->
+    ept C nil K
+| ept_Rf :
+  forall {C: ndctx} {P: o},
+    positive P ->
+    rfc C P ->
+    ept C nil P
+| ept_boxL :
+  forall {C: ndctx} {L: octx} (B: o) {K: o},
+    bracketable K ->
+    permeable B ->
+    ept (ndctx_insert B C) L K ->
+    ept C (B :: L) K
+| ept_AndPL :
+  forall {C: ndctx} {L: octx} (B1 B2 : o) {K: o},
+    bracketable K ->
+    ept C (B2 :: B1 :: L) K ->
+    ept C ((AndP B1 B2) :: L) K
+| ept_OrL :
+  forall {C: ndctx} {L: octx} (B1 B2 : o)  {K: o},
+    bracketable K ->
+    ept C (B1 :: L) K ->
+    ept C (B2 :: L) K ->
+    ept C ((Or B1 B2) :: L) K
+| ept_TrueL :
+  forall {C: ndctx} {L: octx} {K: o},
+    bracketable K ->
+    ept C L K ->
+    ept C (TT :: L) K
+| ept_FalseL :
+  forall {C: ndctx} {L: octx} {K: o},
+    bracketable K ->
+    ept C (FF :: L) K
+with lfc : ndctx -> o -> o -> Prop :=
+| lfc_Rl :
+  forall {C : ndctx} {P : o}  {K : o},
+    bracketable K ->
+    positive P ->
+    ept C (P :: nil) K ->
+    lfc C P K
+| lfc_Il :
+  forall {C: ndctx} {N : o},
+    negative N ->
+    atomic N ->
+    lfc C N N
+| lfc_AndNL_1 :
+  forall {C: ndctx} {B1 B2 : o}  {K : o},
+    bracketable K ->
+    lfc C B1 K ->
+    lfc C (AndN B1 B2) K
+| lfc_AndNL_2 :
+  forall {C: ndctx} {B1 B2 : o}  {K : o},
+    bracketable K ->
+    lfc C B2 K ->
+    lfc C (AndN B1 B2) K
+| lfc_ImpL :
+  forall {C: ndctx} {B1 B2 : o}  {K : o},
+    bracketable K ->
+    rfc C B1 ->
+    lfc C B2 K ->
+    lfc C (Imp B1 B2) K
+with rfc : ndctx -> o -> Prop :=
+| rfc_Rr :
+  forall {C: ndctx} {N: o},
+    negative N ->
+    bct C nil N ->
+    rfc C N
+| rfc_Ir :
+  forall {C: ndctx} {P: o},
+    In P (ndctx_list C) ->
+    positive P ->
+    atomic P ->
+    rfc C P
+| rfc_AndPR :
+  forall {C: ndctx} {B1 B2: o},
+    rfc C B1 ->
+    rfc C B2 ->
+    rfc C (AndP B1 B2)
+| rfc_OrR_1 :
+  forall {C: ndctx} {B1 B2: o},
+    rfc C B1 ->
+    rfc C (Or B1 B2)
+| rfc_OrR_2 :
+  forall {C: ndctx} {B1 B2: o},
+    rfc C B2 ->
+    rfc C (Or B1 B2)
+| rfc_TrueR :
+  forall {C: ndctx},
+    rfc C TT
+.
